wip

research/src/Scratch.v
@@ -3,9 +3,11 @@ Require Import Logic.Decidable.
 Set Implicit Arguments.
 Set Asymmetric Patterns.
 
+
 Inductive Term : Set := 
     | NumTerm : nat -> Term
     | Plus : Term -> Term -> Term
+    | Var : nat -> Term
     .
 
 Fixpoint termDenote (t : Term) : nat := 
@@ -14,7 +16,7 @@ match t with
 | Plus n n' => (termDenote n) + (termDenote n')
 end.
 
-Eval simpl in termDenote (Plus (Plus (NumTerm 0) (NumTerm 5)) (NumTerm 7)).
+Compute termDenote (Plus (Plus (NumTerm 0) (NumTerm 5)) (NumTerm 7)).
 
 Inductive RelOp : Set := 
     | Eq
@@ -29,32 +31,68 @@ match r with
 | Lte => le
 end.
 
+Lemma rels_are_decidable : forall (p : Prop) (r: RelOp) (n1 n2 : nat), (relOpDenote r) n1 n2  = p -> decidable p.
+Proof.
+    intros. destruct r; unfold decidable in *; crush.
+Qed.
+
+Lemma conj_decidable : forall (p1 p2 : Prop), decidable p1 /\ decidable p2 -> decidable (p1 /\ p2).
+Proof. intros. crush. Qed.
+
+
 Inductive Formula : Set := 
+    | Rel : Term -> RelOp -> Term -> Formula
     | And : Formula -> Formula -> Formula
     | Or : Formula -> Formula -> Formula
     | Not : Formula -> Formula
     | ForAll : (nat -> Formula) -> Formula
     | Exists : (nat -> Formula) -> Formula
-    | Rel : Term -> RelOp -> Term -> Formula
     .
+
+Check Exists (fun x : nat => Rel (NumTerm 7) Lte (NumTerm x)).
+
+
+
+
+Definition quantifier_free (f: Formula) : bool :=
+    match f with 
+    | ForAll _ => false
+    | Exists _  => false
+    | _ => true
+    end.
+
+Check forall n : nat, n = n.
+
+Definition EliminateQuantifier (f : nat -> Formula) : Formula * Prop. Admitted.
+
+Fixpoint Cooper (f : ) : Prop :=
+match f with
+| Exists f' => 
 
 Fixpoint formDenote (f : Formula) : Prop := 
 match f with
+    | Rel t1 rel t2 => (relOpDenote rel) (termDenote t1) (termDenote t2)
     | And f1 f2 => (formDenote f1) /\ (formDenote f2)
     | Or f1 f2 => (formDenote f1) \/ (formDenote f2)
     | Not f1 => ~ (formDenote f1)
-    | Rel t1 rel t2 => (relOpDenote rel) (termDenote t1) (termDenote t2)
     | ForAll f' => forall n : nat, formDenote (f' n)
     | Exists f' => exists n : nat, formDenote(f' n)
 end.
 
-Theorem formulas_are_decidable : forall (f : Formula) (p : Prop),
+Hint Resolve rels_are_decidable.
+
+Theorem quantifier_free_formulas_are_decidable : forall (f : Formula) (p : Prop),
+  quantifier_free f = true ->
   formDenote f = p ->
   decidable p.
 Proof.
-intros f.
-induction f.
-- crush.
-- crush.
-- crush.
-- simpl. intros. apply p in H.
+intros f. induction f; eauto; intros; crush.
+Qed.
+
+
+
+
+Theorem formulas_are_decidable : forall (f : Formula) (p : Prop),
+Proof.
+Admitted.
+
